Fact_rec reproved; WIP ewp tactics

coq-osiris/examples/proofs/fact_rec.v
@@ -63,7 +63,10 @@ Definition let_spec {Σ} (module_val : val) (name : var) (spec : val -> iProp Σ
   (* The module value must be a [VStruct]. *)
   match module_val with | VStruct l => _let_spec l | _ => False end.
 
+From osiris.program_logic Require Import ewp protocols protocol_instance.
+
 Section fact_rec_example.
+
   Context `{!osirisGS Σ}.
 
   (** *Factorial specification and proof *)
@@ -98,11 +101,140 @@ Section fact_rec_example.
         [ rewrite eq_repr_repr ; [ done | representable | representable ] | ])
     end).
 
-  (* IY: For now, we're using the old [wp] tactics that we would like to revamp.. *)
-  Example fact_rec_5_correct :
-    ⊢ WP fact_rec_5 {{ RET v, fact_rec_5_spec v }}.
+  Opaque prot_bottom.
+
+  Definition fmap {A B E} (f : A -> B) (m : micro A E) : micro B E :=
+    bind m (fun x => ret (f x)).
+
+  Definition eq_fmap {A B E} (f : A -> B) (m : micro A E) :
+    bind m (fun x => ret (f x)) = fmap f m.
+  Proof. done. Qed.
+
+  Lemma eq_bind_bind {A B E E'} m
+    (k k' : outcome2 B E' → micro A E) :
+    (∀ o, k o = k' o) →
+    bind m k = bind m k'.
   Proof.
+    intros. f_equal.
+    eapply FunctionalExtensionality.functional_extensionality; done.
+  Qed.
+
+  (** *Fmap rule *)
+  Lemma ewp_fmap {A B X} E (f : A -> B) (m : micro A X) Ψ Φ :
+    EWP m @ E <| Ψ |> {{ RET v, Φ (f v) }} -∗
+    EWP fmap f m @ E <| Ψ |> {{ RET v, Φ v }}.
+  Proof.
+    iIntros "Hwp". rewrite -eq_fmap. iApply ewp_bind.
+    iApply (ewp_mono with "[$]"). iIntros (?) "H".
+    destruct a; last done. cbn.
+    iApply ewp_value; by cbn.
+  Qed.
+
+  Example fact_rec_5_correct :
+    ⊢ EWP fact_rec_5 <| prot_bottom |> {{ RET v, fact_rec_5_spec v }}.
+  Proof.
+    iStartProof; rewrite /fact_rec_5. simpl.
+    Par.
+    repeat (simpl_fact; Simp; Try; try Bind).
+
+    simpl_fact; Simp.
+
+    repeat (Ret; cbn).
+    iPureIntro.
+
+    match goal with
+      | |- VInt ?i = VInt (repr ?x) => assert (i = repr x) as ->
+    end.
+    { rewrite !mul_repr_repr; f_equiv. lia. }
+    done.
   Admitted.
+
+  (* Naive :
+
+      Finished transaction in 11.607 secs (11.294u,0.312s) (successful) *)
+
+  (* TODO: Better tactics for [EWP]. *)
+  Example fact_rec_5_correct_opt :
+    ⊢ EWP fact_rec_5 <| prot_bottom |> {{ RET v, fact_rec_5_spec v }}.
+  Proof.
+    iStartProof; rewrite /fact_rec_5. simpl.
+
+    (* Normalization 1 : Normalize bind ("head normal form") *)
+    setoid_rewrite eq_par_par; cycle 1.
+    { intros; rewrite !bind_bind; cbn. reflexivity. }
+
+    (* Normalization 2 : Normalize bind using unit rule and manual rewrite.. *)
+    (* setoid_rewrite eq_par_par; cycle 1. *)
+    (* { intros; rewrite !bind_bind. *)
+
+      (* destruct o; cbn. *)
+      (* { destruct a. rewrite bind_ret. *)
+      (*   Unshelve. *)
+      (*   2 : exact (fun o => *)
+      (*    match o with *)
+      (*    | O2Ret (v, e) => *)
+      (*       ret (VStruct *)
+      (*         (app (cons (pair "fact_rec_5" v) e) *)
+      (*            (cons (pair "fact_rec" (VCloRec nil __bindings2 "fact_rec")) nil))) *)
+      (*    | O2Throw  e => throw e *)
+      (*    end). *)
+      (* reflexivity. } *)
+      (* reflexivity. } *)
+
+    Par.
+
+    (* Normalization 3 *)
+    rewrite try2_join2. cbn. (* [cbn] results in a more efficient term than [Simp]. *)
+
+    (* The exceptional continuation is equivalent to [throw], but only using
+      functional extensionality *)
+    match goal with
+      | |- context[try _ _ ?k] =>
+        replace k with (fun e => throw (A := val) (E := exn) e);
+        [ | apply FunctionalExtensionality.functional_extensionality;
+          reflexivity ]
+    end.
+
+    Simp. rewrite eq_fmap. iApply ewp_fmap.
+
+    repeat (
+    simpl_fact; Simp;
+    rewrite -bind_as_try2 eq_fmap;
+    iApply ewp_fmap;
+    iApply ewp_bind).
+
+    simpl_fact; Simp.
+
+    repeat (Ret; cbn).
+    iPureIntro.
+
+    match goal with
+      | |- VInt ?i = VInt (repr ?x) => assert (i = repr x) as ->
+    end.
+    { rewrite !mul_repr_repr; f_equiv. lia. }
+    done.
+  Time Qed.
+
+  (* With normalization 1:
+
+      Finished transaction in 6.723 secs (6.503u,0.219s) (successful) *)
+
+  (* With normalization 2:
+
+      Finished transaction in 6.498 secs (6.305u,0.192s) (successful) *)
+
+  (* With normalization 2 + 3:
+
+      Finished transaction in 4.443 secs (4.338u,0.105s) (successful)
+   *)
+
+  (* With 2 + 3 + FMap :
+
+      Finished transaction in 0.972 secs (0.945u,0.027s) (successful) *)
+
+  (* With 1 + 3 + FMap :
+
+      Finished transaction in 0.94 secs (0.914u,0.025s) (successful) *)
 
   (* --------------------------------------------------------------------- *)
   (* Next is the specification of the stateful implementation of factorial. *)
@@ -120,9 +252,51 @@ Section fact_rec_example.
     let _spec v := (⌜v = # 120⌝)%I in
     let_spec v "fact_5" _spec.
 
+  (* TODO: Term explosion is really not great *)
   Example fact_5_correct :
-    ⊢ WP fact_5 {{ RET v, fact_5_spec v }}.
+    ⊢ EWP fact_5 <| prot_bottom |> {{ RET v, fact_5_spec v }}.
   Proof.
+    iStartProof.
+    rewrite /fact_rec_5 /eval_mexpr; cbn.
+    Par; cbn.
+
+    (* Allocate a new variable that stores the dummy function value *)
+    Alloc factv "Hfact".
+
+    Simp.
+
+    (* We store the value of [fact0] that ties the recursive knot. *)
+    Store "Hfact".
+    iIntros "Hfactv".
+
+    Simp.
+
+    simpl_fact. Try. Simp. cbn.
+    repeat (simpl_fact; Try; Bind; Simp).
+
+    repeat (Ret; cbn).
+    Par.
+
+    (* Reduce each call to [fact] *)
+    Try. simpl_fact. Simp.
+    ewp_tactics.Load "Hfactv". iIntros "Hfactv".
+
+    repeat (
+    Try; Bind; cbn; Simp;
+    simpl_fact; Simp;
+    ewp_tactics.Load "Hfactv"; iIntros "Hfactv").
+
+    Try. Bind. cbn. Simp.
+    simpl_fact; Simp.
+
+    repeat (Ret; cbn).
+
+    iPureIntro.
+    match goal with
+      | |- VInt ?i = VInt (repr ?x) => assert (i = repr x) as ->
+    end.
+    { rewrite !mul_repr_repr; f_equiv. lia. }
+    done.
   Admitted.
 
 End fact_rec_example.
@@ -138,24 +312,3 @@ End fact_rec_example.
            => the reasoning will be pushed down to [pure] for [fact_rec]
 
      (2) Prove a simulation between [fact_rec] and [fact], ignoring store *)
-
-(* --------------------------------------------------------------------- *)
-
-From iris Require Import program_logic.adequacy.
-From osiris Require Import program_logic.adequacy.
-
-(** * Adequacy sanity check
-
-  Instantiating concrete example program for adequacy
-
-  Following instantiation of a concrete program in heap_lang; see
-  https://gitlab.mpi-sws.org/iris/iris/-/blob/master/tests/one_shot.v?ref_type=heads *)
-
-Lemma client_adequate σ :
-  adequate NotStuck fact_5 σ (λ v _, True).
-Proof.
-Admitted.
-
-(* Print Assumptions client_adequate. *)
-(* Some assumptions about integers, funext and eqdep.
-    Free of iris-related assumptions. *)
