coq-osiris/theories/proofmode/ewp_tactics.v
@@ -119,3 +119,4 @@ Global Hint Extern 0 (envs_entails _ (bi_forall (fun _ : void => _))) => iIntros
 Global Hint Extern 0 (envs_entails _ (ewp_def _ (ret _) _ _)) => ewp: Ret : core.
 
 Notation "OCAML⟦ x ⟧" := (eval.eval (deco x _)).
+
